theories/interp.v
@@ -774,10 +774,86 @@ Section proofs.
         by lia.
   Qed.
 
-  Lemma iForall3_interp_equivI (Σ0 Σ1 : list (interp Θ)):
+  Lemma interp_type_pre_app ty: ∀ Σ0 Σ1,
+    bounded (length Σ0) ty →
+    interp_type_pre interp_type ty Σ0 ≡
+    interp_type_pre interp_type ty (Σ0 ++ Σ1).
+  Proof.
+    induction ty as [ | | | | A σ hi | | | A B hA hB | A B hA hB | i
+    | cname | | ] => Σ0 Σ1 hb w //=.
+    - rewrite !interp_tag_unseal /interp_tag_def /interp_fun !interp_car_simpl.
+      do 17 f_equiv.
+      { rewrite !fmap_length. 
+        by repeat f_equiv.
+      }
+      f_equiv.
+      { do 10 f_equiv.
+        assert (hm:
+          interp_type MixedT (go interp_type Σ0 <$> σ) a9 ⊣⊢
+          interp_type MixedT (go interp_type (Σ0 ++ Σ1) <$> σ) a9)
+        by by rewrite !interp_mixed_unfold.
+        done.
+      }
+      do 16 f_equiv.
+      rewrite Forall_lookup in hi.
+      rewrite !list_lookup_fmap.
+      destruct (σ !! a7) as [ty | ] eqn:hty; last done.
+      apply hi with (Σ0 := Σ0) (Σ1 := Σ1) in hty; last first.
+      { inv hb.
+        rewrite Forall_lookup in H0.
+        by eauto.
+      }
+      simpl in *.
+      by rewrite hty.
+    - inv hb.
+      f_equiv.
+      + by apply hA with (Σ1 := Σ1) in H1.
+      + by apply hB with (Σ1 := Σ1) in H2.
+    - inv hb.
+      f_equiv.
+      + by apply hA with (Σ1 := Σ1) in H1.
+      + by apply hB with (Σ1 := Σ1) in H2.
+    - inv hb.
+      by rewrite /interp_generic lookup_app_l.
+  Qed.
+
+  Lemma interp_type_app ty: ∀ Σ0 Σ1,
+    bounded (length Σ0) ty →
+    interp_type ty Σ0 ≡
+    interp_type ty (Σ0 ++ Σ1).
+  Proof.
+    move => Σ0 Σ1 hb v.
+    by rewrite !interp_type_unfold interp_type_pre_app.
+  Qed.
+
+  Lemma iForall3_interp_equivI_l (Σ0 Σ1 : list (interp Θ)):
     Σ0 ≡ Σ1 →
     ∀ vs Σ,
     iForall3 interp_variance vs Σ0 Σ ≡ iForall3 interp_variance vs Σ1 Σ.
+  Proof.
+    move => heq vs.
+    assert (hl: length Σ0 = length Σ1) by by rewrite heq.
+    move : Σ0 Σ1 heq hl.
+    induction vs as [ | v vs hi] => Σ0 Σ1 heq hl Σ.
+    { by destruct Σ0; destruct Σ1; destruct Σ. }
+    destruct Σ0 as [ | i0 Σ0] => //=.
+    { symmetry in hl.
+      by apply nil_length_inv in hl; rewrite hl.
+    }
+    destruct Σ1 as [ | i1 Σ1] => //=.
+    destruct Σ as [ | i Σ] => //=.
+    case : hl => hl.
+    apply cons_equiv_eq in heq as (i1' & Σ1' & [= -> ->] & h0 & h1).
+    f_equiv.
+    - rewrite /interp_variance.
+      by repeat f_equiv.
+    - by rewrite (hi _ _ h1 hl Σ).
+  Qed.
+
+  Lemma iForall3_interp_equivI_r (Σ0 Σ1 : list (interp Θ)):
+    Σ0 ≡ Σ1 →
+    ∀ vs Σ,
+    iForall3 interp_variance vs Σ Σ0 ≡ iForall3 interp_variance vs Σ Σ1.
   Proof.
     move => heq vs.
     assert (hl: length Σ0 = length Σ1) by by rewrite heq.
@@ -808,6 +884,40 @@ Section proofs.
     - by iApply hi.
   Qed.
 
+  Lemma interp_type_rigid Σ0 Σ1 t:
+    map_Forall (λ _ : string, wf_cdef_parent pdefs) pdefs →
+    wf_ty (ClassT t (map GenT (seq (length Σ0) (length Σ1)))) →
+    interp_tag interp_type Σ1 t ≡
+    interp_type (ClassT t (map GenT (seq (length Σ0) (length Σ1)))) (Σ0 ++ Σ1).
+  Proof.
+    move => hp hwf v.
+    rewrite interp_tag_equiv; last done.
+    rewrite interp_class_unfold => //.
+    rewrite /interp_tag_alt /=.
+    do 17 f_equiv.
+    { by rewrite /interp_list !fmap_length seq_length. }
+    do 5 f_equiv.
+    assert (h : interp_list (Σ0 ++ Σ1) (map GenT (seq (length Σ0) (length Σ1))) ≡ Σ1).
+    { rewrite /interp_list.
+      apply list_equiv_lookup => k.
+      rewrite !list_lookup_fmap.
+      destruct (Σ1 !! k) as [ϕ | ] eqn:heq; last first.
+      { rewrite heq.
+        apply lookup_ge_None_1 in heq.
+        by rewrite lookup_seq_ge.
+      }
+      rewrite lookup_seq_lt; last first.
+      { apply mk_is_Some in heq.
+        by apply lookup_lt_is_Some_1 in heq.
+      }
+      rewrite /= heq; f_equiv => w.
+      rewrite interp_generic_unfold /interp_generic lookup_app_r; last by lia.
+      replace (length Σ0 + k - length Σ0) with k by lia.
+      by rewrite heq.
+    }
+    by rewrite (iForall3_interp_equivI_r _ _ h).
+  Qed.
+
   Lemma iForall3_interp_gen_targs vs n Σ:
     length vs = n →
     length Σ = n →
@@ -829,7 +939,7 @@ Section proofs.
         rewrite /gen_targs !list_lookup_fmap /= lookup_seq_ge //.
         by lia.
     }
-    rewrite (iForall3_interp_equivI _ _ heq).
+    rewrite (iForall3_interp_equivI_l _ _ heq).
     apply iForall3_interp_reflexive => //.
     by rewrite hl0.
   Qed.
@@ -1146,7 +1256,7 @@ Section proofs.
       rewrite H2.
       by apply hF.
     }
-    rewrite (iForall3_interp_equivI _ _ heq bdef.(generics) (interp_list Σ σB)).
+    rewrite (iForall3_interp_equivI_l _ _ heq bdef.(generics) (interp_list Σ σB)).
     iApply (interp_env_with_mono with "hinst") => //.
     + by apply wf_ty_class_inv in hwfB.
     + inv hwfB; by simplify_eq.
@@ -1495,11 +1605,52 @@ Section proofs.
   Definition interp_this_type C (σC: list lang_ty) Σ : interp Θ :=
     interp_this C (interp_list Σ σC).
 
+  Lemma interp_this_type_app C σC: ∀ Σ0 Σ1,
+    bounded (length Σ0) (ClassT C σC) →
+    interp_this_type C σC Σ0 ≡
+    interp_this_type C σC  (Σ0 ++ Σ1).
+  Proof.
+    move => Σ0 Σ1 hb w.
+    rewrite /interp_this_type !interp_this_unseal /interp_this_def /interp_fun !interp_car_simpl.
+    do 17 f_equiv.
+    { rewrite !fmap_length. 
+      by repeat f_equiv.
+    }
+    do 4 f_equiv.
+    rewrite /interp_list.
+    apply list_fmap_equiv_ext_elem_of => ty hty.
+    apply interp_type_app.
+    inv hb.
+    rewrite Forall_forall in H0.
+    by apply H0.
+  Qed.
+
   Definition interp_local_tys Σ
     (Γ : local_tys) (le : local_env) : iProp Θ := 
     interp_this_type Γ.(type_of_this).1 Γ.(type_of_this).2 Σ (LocV le.(vthis)) ∗
     (∀ v ty, ⌜Γ.(ctxt) !! v = Some ty⌝ -∗
     ∃ val, ⌜le.(lenv) !! v = Some val⌝ ∗ interp_type ty Σ val)%I.
+
+  Lemma interp_local_app Γ st Σ0 Σ1:
+    bounded_lty (length Σ0) Γ →
+    interp_local_tys Σ0 Γ st ≡
+    interp_local_tys (Σ0 ++ Σ1) Γ st.
+  Proof.
+    move => hb.
+    rewrite /interp_local_tys.
+    f_equiv.
+    - rewrite -interp_this_type_app; first done.
+      by apply hb.
+    - iStartProof; iSplit; iIntros "h"; iIntros (v ty hv).
+      + iDestruct ("h" $! v ty hv) as (w hw) "#hw".
+        iExists w; iSplit; first done.
+        rewrite -interp_type_app; first done.
+        by apply hb in hv.
+      + iDestruct ("h" $! v ty hv) as (w hw) "#hw".
+        iExists w; iSplit; first done.
+        rewrite -interp_type_app; first done.
+        by apply hb in hv.
+  Qed.
 
   Lemma interp_local_tys_is_inclusion kd Σ Γ0 Γ1 le:
     wf_lty Γ0 →
@@ -1526,31 +1677,6 @@ Section proofs.
     iExists val; iSplitR; first done.
     iApply subtype_is_inclusion => //.
     by apply hlty in hB.
-  Qed.
-
-  (* Specialized version for existential types. Will help during the
-   * proof of soundness for runtime checks.
-   *)
-  Theorem inherits_is_ex_inclusion Σ:
-    ∀ A B, inherits A B →
-    ∀ v, interp_type (ExT A) Σ v -∗ interp_type (ExT B) Σ v.
-  Proof.
-    induction 1 as [ x | x y z hxy hyz hi ] => // v.
-    rewrite interp_ex_unfold.
-    iIntros "H".
-    iApply hi; clear hyz hi.
-    iDestruct "H" as (Σx) "H".
-    destruct hxy as [x y xdef' σy hxdef' hsuper]; simplify_eq.
-    assert (hext: extends_using x y σy) by (econstructor; by eauto).
-    rewrite (interp_tag_equiv x) //.
-    iDestruct ((tag_extends_using_is_inclusion wf_parent wf_mono x y σy) with "H") as "H" => //.
-    rewrite interp_ex_unfold /interp_ex /=.
-    apply wf_parent in hxdef'.
-    rewrite /wf_cdef_parent hsuper in hxdef'.
-    destruct hxdef' as [hwf _].
-    inv hwf.
-    iExists (interp_list Σx σy).
-    by rewrite (interp_tag_equiv y).
   Qed.
   End Inclusion.
 End proofs.
